TLam, TApp, TOpen rules

coqsrc/Explicit/MTypeRules.v
@@ -2,6 +2,7 @@ Require Import Utf8.
 Require Import Common.MBinder.
 Require Import Explicit.MSyntax.
 Require Import Explicit.ExplicitKind.
+Require Import Coq.Lists.List.
 
 (* 2329 〈  232a 〉 *)
 
@@ -103,7 +104,37 @@ Definition env_ext {W:world} {TV : Set} {V :Set}
 
 Notation "Γ ',+' τ" := (@env_ext _ _ _ Γ τ) (at level 45, left associativity).
 
+Fixpoint inc_type {W:world} {TV : Set} (τ : typ W TV) : typ W (inc TV).
+Proof.
+  remember (@inc_type W TV) as Inc.
+  destruct τ eqn:τ_eqn.
+  + apply (t_var (VS t)).
+  + apply (t_base w).
+  + apply (t_effect w (map Inc l)).
+  + apply (〈〉).
+  + apply (〈Inc t1 | Inc t2〉).
+  + apply ( Inc t1 ==>[Inc t2] Inc t3).
+  + apply (t_forall k (@inc_type W (inc TV) t)).
+Defined.
+
+Definition inc_env {W:world} {TV : Set} {V :Set} (Γ : @env W TV V) (x : V) : typ W (inc TV) :=
+  inc_type (Γ x).
+
+Definition kinding_env_ext {TV : Set}
+  (Δ:TV → kind) (k : kind) (α : inc TV) : kind :=
+  match α with
+  | VZ    => k
+  | VS α' => Δ α'
+  end.
+
+Notation "Δ ',*' k" := (@kinding_env_ext _ Δ k) (at level 45, left associativity).
+
 Reserved Notation "Γ ';' Δ '⊢' t '∈' τ '|' ε" (at level 50).
+
+Fixpoint open_row_with {W:world} {TV : Set} {Δ : TV → kind}
+  (ls: typ W TV) (ls_s : ls ::[Δ] k_eff_row)
+  (ε : typ W TV) (ε_s  : ε  ::[Δ] k_eff_row) : typ W TV.
+Admitted. 
 
 Inductive has_type {W:world} {TV : Set} {V : Set} (Γ : @env W TV V) (Δ : TV → kind): 
   expr W TV V → typ W TV → typ W TV → Prop :=
@@ -117,23 +148,45 @@ Inductive has_type {W:world} {TV : Set} {V : Set} (Γ : @env W TV V) (Δ : TV �
     Γ ; Δ ⊢ v_const b v ∈ t_base b | ε
 | T_Var : ∀ (x : V) (ε : typ W TV),
     ε ::[Δ] k_eff_row →
-    Γ ; Δ  ⊢ v_var x ∈ (Γ x) | ε
+    Γ ; Δ ⊢ v_var x ∈ (Γ x) | ε
 
-| T_Lam : ∀ (e : expr W TV (inc V)) (σ σ₁ ε ε' STH: typ W TV),
+| T_Lam : ∀ (e : expr W TV (inc V)) (σ σ₁ ε ε': typ W TV),
     σ  ::[Δ] k_type →
     σ₁ ::[Δ] k_type →
     ε  ::[Δ] k_eff_row →
     ε' ::[Δ] k_eff_row →
     Γ,+ σ₁ ; Δ  ⊢ e ∈ σ | ε → 
-    Γ ; Δ  ⊢ v_lam σ₁ e ε ∈ σ₁ ==>[ε] σ | ε'
+    Γ ; Δ ⊢ v_lam σ₁ e ε ∈ σ₁ ==>[ε] σ | ε'
 
 | T_App : ∀ (e₁ e₂ : expr W TV V) (σ σ₂ ε : typ W TV),
     σ  ::[Δ] k_type →
     σ₂ ::[Δ] k_type →
     ε  ::[Δ] k_eff_row →
-    Γ ; Δ  ⊢ e₁ ∈ σ₂ ==>[ε] σ | ε →
-    Γ ; Δ  ⊢ e₂ ∈ σ₂ | ε →
-    Γ ; Δ  ⊢ e_app e₁ e₂ ∈ σ | ε
+    Γ ; Δ ⊢ e₁ ∈ σ₂ ==>[ε] σ | ε →
+    Γ ; Δ ⊢ e₂ ∈ σ₂ | ε →
+    Γ ; Δ ⊢ e_app e₁ e₂ ∈ σ | ε
+
+| T_TLam : ∀ (e: value W (inc TV) V) (σ: typ W (inc TV)) (ε: typ W TV) (k :kind),
+    σ  ::[Δ,* k] k_type  →
+    ε  ::[Δ] k_eff_row →
+    inc_env Γ ; (Δ,* k)  ⊢ e ∈ σ | inc_type ε →
+    Γ ; Δ ⊢ v_tlam k e ∈ t_forall k σ | ε 
+
+| T_TApp : ∀ (e : expr W TV V) (σ₁ ε : typ W TV) (σ : typ W (inc TV)) (k :kind),
+    σ₁ ::[Δ] k_type →
+    ε  ::[Δ] k_eff_row →
+    σ  ::[Δ,* k] k_type →
+    Γ ; Δ ⊢ e ∈ t_forall k σ | ε →
+    Γ ; Δ ⊢ e_tapp e σ₁ ∈ tsubst_t σ σ₁ | ε
+
+| T_Open : ∀ (e : expr W TV V) (σ₁ σ₂ ls ε ε' : typ W TV)
+    (ls_s : ls  ::[Δ] k_eff_row)
+    (ε_s  : ε   ::[Δ] k_eff_row),
+    σ₁  ::[Δ] k_type →
+    σ₂  ::[Δ] k_type →
+    ε'  ::[Δ] k_eff_row →
+    Γ ; Δ ⊢ e ∈ σ₁ ==>[ls] σ₂ | ε' →
+    Γ ; Δ ⊢ e_open e ε ∈ σ₁ ==>[open_row_with ls ls_s ε ε_s] σ₂ | ε'
 
 | T_Let : ∀ (e₁ : expr W TV V) (e₂ : expr W TV (inc V)) (σ σ₂ ε : typ W TV),  
     σ  ::[Δ] k_type →
